finish fsub/autosubst2 subtyping_transitivity and subtyping_narrowing

fsub/autosubst2_dctx/prop_subtyping.v
@@ -2,19 +2,138 @@ Require Import common.prop_as_core.
 Require Import common.prop_as_unscoped.
 Require Import fsub.autosubst2_dctx.def_as2.
 Require Import fsub.autosubst2_dctx.def_extra.
+Require Import fsub.autosubst2_dctx.prop_basic.
 
 From Coq Require Import ssreflect ssrfun ssrbool.
 From Hammer Require Import Tactics.
 Require Import Coq.Program.Equality.
+Require Import Nat.
 Require Import List.
+Require Import Arith.
 
 Import SubstNotations.
 Import UnscopedNotations.
 
-Theorem subtyping_reflexivity Δ A : 
-  Δ ⊢ A ->
-  Δ ⊢ A <: A.
+Fixpoint typ_size (A : typ) :=
+  match A with
+  | typ_arr A B => 1 + typ_size A + typ_size B
+  | typ_all A B => 1 + typ_size A + typ_size B
+  | _ => 0
+  end.
+
+Lemma typ_size_renaming_eq A ξ:
+  typ_size (A ⟨ ξ ⟩) = typ_size A.
 Proof.
-  move : Δ; elim: A; intros; try hauto ctrs:subtyping.
-  apply sub_top; eauto.
+  move : ξ; induction A; intros; simpl; hauto.
+Qed.
+
+Lemma lookup_tvar_det : forall Δ X A B,
+  lookup_tvar X Δ A -> lookup_tvar X Δ B -> A = B.
+Proof.
+  intros. move : B H0. 
+    induction H; hauto inv:lookup_tvar ctrs:lookup_tvar.
+Qed.
+
+Corollary ctx_tvar_renaming_tvars Δ1 Δ2 A: 
+  ctx_tvar_rename Δ1 (Δ2 ++ A :: Δ1) (fun X : nat => 1 + (length Δ2 + X)).
+Proof.
+  intros. unfold ctx_tvar_rename. intros.
+    induction Δ2; simpl; try hauto inv:lookup_tvar ctrs:lookup_tvar.
+  - replace (⟨fun X0 : nat => S (S (length Δ2 + X0))⟩ B) with
+    (B ⟨fun X : nat => 1 + (length Δ2 + X)⟩ ⟨ ↑⟩ ) by (asimpl; auto).
+    hauto ctrs:lookup_tvar.
+Qed.
+
+
+Lemma lookup_tvar_rebounding : forall Δ1 Δ2 B,
+  lookup_tvar (length Δ2) (Δ2 ++ B :: Δ1) (B ⟨fun X => 1 + (length Δ2 + X) ⟩) /\
+  (forall X A B', X <> length Δ2 -> 
+    lookup_tvar X (Δ2 ++ B :: Δ1) A ->
+    lookup_tvar X (Δ2 ++ B' :: Δ1) A).
+Proof.
+  split. 
+  - induction Δ2; simpl; asimpl; try hauto ctrs:lookup_tvar.
+    + replace (ren_typ (fun X : nat => S (S (length Δ2 + X))) B) with
+      (B ⟨fun X : nat => 1 + (length Δ2 + X)⟩ ⟨ ↑⟩ ) by (asimpl; auto).
+      hauto ctrs:lookup_tvar.
+  - intros. dependent induction H0.
+    + destruct Δ2; simpl in *; try hauto ctrs:lookup_tvar.
+    + destruct Δ2; simpl in *; try hauto ctrs:lookup_tvar.
+Qed.
+
+Lemma conj' (A B : Prop) : A -> (A -> B) -> A /\ B.
+Proof. tauto. Qed.
+
+Theorem subtyping_transitivity_narrowing n:
+  (forall Δ A B C,  
+    typ_size B = n -> 
+    Δ ⊢ A <: B ->
+    Δ ⊢ B <: C ->
+    Δ ⊢ A <: C) /\
+  (forall Δ1 Δ2 A B B' C,
+    typ_size B = n -> 
+    Δ2 ++ (B :: Δ1) ⊢ A <: C ->
+    Δ1 ⊢ B' <: B ->
+    Δ2 ++ (B' :: Δ1) ⊢ A <: C).
+Proof.
+  induction (lt_wf n) as [n _ IH].
+  intros. apply conj'.
+  - intros. move : C H1. induction H0; intros; try hauto ctrs:subtyping.
+      + inversion H1; subst.
+        * hauto ctrs:subtyping. 
+      + simpl in *. 
+        inversion H1; subst.
+        * eapply sub_top. hauto use:sub_wf_typ1, sub_wf_typ2.
+        * eapply sub_arrow.
+          --  edestruct (IH (typ_size B1)). hfcrush. hauto. 
+          --  edestruct (IH (typ_size B2)). hfcrush. hauto. 
+      + inversion H1; subst.
+        * eapply sub_top. simpl in *. split.
+          -- hauto use:sub_wf_typ1, sub_wf_typ2.
+          -- eapply wf_typ_renaming_tvar' with (ξ:=id) (A:=A2) (A':=A2) (Δ:=B1::Δ);
+            hauto unfold:ctx_tvar_rename_weak inv:lookup_tvar ctrs:lookup_tvar use:sub_wf_typ1, sub_wf_typ2 simp+:asimpl.
+        * eapply sub_all; eauto.
+          -- edestruct (IH (typ_size B1)). hfcrush. auto. hauto. 
+          -- edestruct (IH (typ_size B1)). eauto. hfcrush. eauto. 
+             edestruct (IH (typ_size B2)). hfcrush. eauto.
+             replace (B0 :: Δ) with (nil ++ B0 :: Δ) by auto.
+             eapply H2; eauto.
+  - intros Htrans. intros. move : B' H1. dependent induction H0; intros; auto.
+    + eapply sub_top.
+      eapply wf_typ_renaming_tvar' with (ξ:=id); 
+        hauto use:ctx_tvar_rename_weak_rebounding simp+:asimpl.
+    + eapply sub_tvar_refl; eauto.
+       eapply wf_typ_renaming_tvar' with (ξ:=id) (A:=typ_var X); 
+        hauto use:ctx_tvar_rename_weak_rebounding simp+:asimpl.
+    + edestruct (Nat.eq_dec X (length Δ2)).
+      * subst. 
+        eapply sub_tvar_bound with (A:=B' ⟨fun X => 1 + (length Δ2 + X) ⟩).
+        hauto use:lookup_tvar_rebounding. eapply Htrans with (B:=B ⟨fun X => 1 + (length Δ2 + X) ⟩).
+        -- hauto use:typ_size_renaming_eq.
+        -- eapply sub_renaming_tvar; eauto.
+           eapply ctx_tvar_renaming_tvars.
+        -- erewrite (lookup_tvar_det _ _ (⟨fun X : nat => 1 + (length Δ2 + X)⟩ B)); eauto.
+           hauto use:lookup_tvar_rebounding.
+      * subst. eapply sub_tvar_bound; eauto.
+        eapply lookup_tvar_rebounding; eauto.
+    + hauto ctrs:subtyping.
+    + eapply sub_all; try hauto ctrs:subtyping.
+      * eapply wf_typ_renaming_tvar' with (ξ:=id); 
+        hauto use:ctx_tvar_rename_weak_rebounding simp+:asimpl.
+      * replace (B1 :: Δ2 ++ B' :: Δ1) with ((B1 :: Δ2) ++ B' :: Δ1) by auto.
+        eapply IHsubtyping2; eauto.
+Qed.
+
+Corollary subtyping_transitivity Δ A B C:
+  Δ ⊢ A <: B -> Δ ⊢ B <: C -> Δ ⊢ A <: C.
+Proof.
+  eapply subtyping_transitivity_narrowing; eauto.
+Qed.
+
+Corollary subtyping_narrowing Δ1 Δ2 A B B' C:
+  Δ2 ++ B :: Δ1 ⊢ A <: C ->
+  Δ1 ⊢ B' <: B ->
+  Δ2 ++ B' :: Δ1 ⊢ A <: C.
+Proof.
+  eapply subtyping_transitivity_narrowing; eauto.
 Qed.
